src/verification/BlockVer/Examples.v
@@ -1,0 +1,127 @@
+From Coq Require Import
+     ZArith.ZArith
+     Lists.List
+     micromega.Lia
+     Strings.String.
+From Katamaran Require Import
+     Notations
+     Bitvector
+     Semantics.
+
+From MSP430 Require Import
+  BlockVer.Spec
+  BlockVer.Verifier
+  Machine
+  Sig.
+
+Import MSP430Program.
+Import MSP430BlockVerifExecutor.
+Import Assembly.
+
+Set Implicit Arguments.
+Import ctx.resolution.
+Import ctx.notations.
+Import bv.notations.
+Import env.notations.
+Import ListNotations.
+Import asn.notations.
+
+Module Examples.
+  Definition asn_mpu_registers {Σ} : Assertion Σ :=
+      ∃ "MPUCTL0_reg"    , MPUCTL0_reg    ↦ term_var "MPUCTL0_reg"
+    ∗ ∃ "MPUCTL1_reg"    , MPUCTL1_reg    ↦ term_var "MPUCTL1_reg"
+    ∗ ∃ "MPUSEGB2_reg"   , MPUSEGB2_reg   ↦ term_var "MPUSEGB2_reg"
+    ∗ ∃ "MPUSEGB1_reg"   , MPUSEGB1_reg   ↦ term_var "MPUSEGB1_reg"
+    ∗ ∃ "MPUSAM_reg"     , MPUSAM_reg     ↦ term_var "MPUSAM_reg".
+
+  Definition minimal_pre {Σ} : Assertion Σ :=
+    ∃ "ipectl", MPUIPC0_reg    ↦ term_var "ipectl" ∗
+    ∃ "segb1" , MPUIPSEGB1_reg ↦ term_var "segb1"  ∗
+    ∃ "segb2" , MPUIPSEGB2_reg ↦ term_var "segb2"  ∗
+    asn_mpu_registers.
+
+  Definition minimal_post {Σ} : Assertion Σ := minimal_pre.
+
+  Definition VC_triple {Σ}
+    (P : Assertion (Σ ▻ "a" :: ty.Address))
+    (i : list ast_with_args)
+    (Q : Assertion (Σ ▻ "a" :: ty.Address ▻ "an" :: ty.Address))
+  :=
+    cblock_verification_condition (minimal_pre ∗ P) i (minimal_post ∗ Q).
+
+
+  Definition Valid_VC {Σ}
+    (P : Assertion (Σ ▻ "a" :: ty.Address))
+    (i : list ast_with_args)
+    (Q : Assertion (Σ ▻ "a" :: ty.Address ▻ "an" :: ty.Address))
+  :=
+    VC_triple P i Q
+    (* safeE (postprocess (VC_triple P i Q)) *).
+
+  (*
+  Definition Debug_VC {Σ}
+    (P : Assertion (Σ ▻ "a" :: ty.Address))
+    (i : list ast_with_args)
+    (Q : Assertion (Σ ▻ "a" :: ty.Address ▻ "an" :: ty.Address))
+  :=
+    VerificationCondition (postprocess (VC_triple P i Q)).
+   *)
+
+  Record BlockVerifierContract {Σ} :=
+    MkBlockVerifierContract
+      { precondition  : Assertion (Σ ▻ "a" :: ty.Address)
+      ; instrs        : list ast_with_args
+      ; postcondition : Assertion (Σ ▻ "a" :: ty.Address ▻ "an" :: ty.Address)
+      }.
+
+  Definition map {Σ A} (c : @BlockVerifierContract Σ)
+    (f : Assertion (Σ ▻ "a" :: ty.Address) -> list ast_with_args -> Assertion (Σ ▻ "a" :: ty.Address ▻ "an" :: ty.Address) -> A)
+    : A :=
+    match c with
+    | {| precondition := pre; instrs := i; postcondition := post |} =>
+        f pre i post
+    end.
+
+  Definition ValidBlockVerifierContract {Σ} (c : @BlockVerifierContract Σ) : Prop :=
+    map c Valid_VC.
+
+  Local Notation "'{{' P '}}' i '{{' Q '}}'" :=
+    (@MkBlockVerifierContract [ctx] P%asn i Q%asn)
+      (at level 90, format "'[v' '{{'  P  '}}' '/'  i '/' '{{'  Q  '}}' ']'").
+
+  Local Ltac solve_bv :=
+      repeat match goal with
+        | |- context[bv.add ?x (@BitvectorBase.bv.mk ?n 0 I)] =>
+            fold (@bv.zero n)
+        | |- context[bv.add ?x bv.zero] =>
+            rewrite BitvectorBase.bv.add_zero_r
+        end.
+
+  Local Ltac solve_vc :=
+    vm_compute; constructor; cbn; intros; repeat split; try solve_bv; auto.
+
+  Definition asn_init_pc {Σ} : Assertion (Σ ▻ "a" :: ty.Address) :=
+    term_var "a" = term_val ty.Address bv.zero.
+
+  Definition ex_mov_register : BlockVerifierContract :=
+    {{
+        asn_init_pc ∗
+        R4_reg ↦ term_val ty.wordBits [bv 42] ∗
+        ∃ "v", R5_reg ↦ term_var "v"
+    }}
+
+    [MOV_WRR R4 R5]
+
+    {{
+        R4_reg ↦ term_val ty.wordBits [bv 42] ∗
+        R5_reg ↦ term_val ty.wordBits [bv 42]
+    }}.
+
+  Example valid_ex_move_register : ValidBlockVerifierContract ex_mov_register.
+  Proof.
+    (* solve_vc. *)
+   vm_compute.
+vm_compute; constructor; cbn; intros; repeat split; try solve_bv; auto
+  Qed.
+
+End Examples.
