src/verification/BlockVer/Spec.v
@@ -1,0 +1,314 @@
+From Coq Require Import
+     ZArith.ZArith
+     Strings.String
+     Lists.List.
+From Equations Require Import
+     Equations.
+From Katamaran Require Import
+     Iris.Instance
+     Iris.Base
+     Notations
+     Bitvector
+     Sep.Hoare
+     Specification
+     MicroSail.ShallowExecutor
+     MicroSail.ShallowSoundness
+     MicroSail.SymbolicExecutor
+     MicroSail.RefineExecutor
+     MicroSail.Soundness.
+
+From MSP430 Require Import Machine Sig.
+
+Import MSP430Program.
+Import ListNotations.
+
+Set Implicit Arguments.
+Import ctx.resolution.
+Import ctx.notations.
+Import env.notations.
+Import bv.notations.
+
+Open Scope string_scope.
+Open Scope ctx_scope.
+Open Scope Z_scope.
+
+Module Assembly.
+  Inductive ast_with_args :=
+  | I0 (i : ast)
+  | I1 (i : ast) (a : bv 16)
+  | I2 (i : ast) (a : bv 16) (b : bv 16).
+
+  Definition instr_without_args i :=
+    match i with
+      I0 i | I1 i _ | I2 i _ _ => i
+    end.
+
+  Definition MOV_WRR (rs rd : Register) : ast_with_args :=
+    I0 (DOUBLEOP MOV WORD_INSTRUCTION rs REGISTER_MODE rd REGISTER_MODE).
+
+  Definition ADD_WRR (rs rd : Register) : ast_with_args :=
+    I0 (DOUBLEOP ADD WORD_INSTRUCTION rs REGISTER_MODE rd REGISTER_MODE).
+End Assembly.
+
+Module MSP430BlockVerifSpec <: Specification MSP430Base MSP430Signature MSP430Program.
+  Include SpecificationMixin MSP430Base MSP430Signature MSP430Program.
+
+  Import asn.notations.
+
+  Local Notation "a @ b" := (term_binop (@bop.bvapp _ 8 8) a b) (at level 60).
+  Local Notation "v +' n" :=  (term_binop bop.bvadd v (term_val ty.wordBits [bv n])) (at level 50).
+
+  Local Notation "a m↦ v" := (asn.chunk (chunk_user ptstomem [a; v])) (at level 70).
+  Local Notation "a i↦ i" := (asn.chunk (chunk_user ptstoinstr [a; i])) (at level 70).
+  Local Notation "w ≡ i" := (asn.chunk (chunk_user encodes_instr [w; i])) (at level 70).
+
+  Local Notation asn_accessible_addresses segb1 segb2 :=
+    (asn.chunk_angelic (chunk_user accessible_addresses
+                          [term_var segb1; term_var segb2])).
+
+  Local Notation asn_accessible_addresses_without segb1 segb2 addr :=
+    (asn.chunk_angelic (chunk_user accessible_addresses_without
+                          [term_var segb1; term_var segb2; term_var addr])).
+
+  Definition term_plus {Σ} (m : Z) (n : Term Σ ty.int) : Term Σ ty.int :=
+    (term_binop bop.plus n (term_val ty.int m)).
+
+  Definition word_times_16 {Σ} (w : Term Σ ty.wordBits) : Term Σ ty.int :=
+    (term_binop bop.times
+       (term_unsigned w)
+       (term_val ty.int 16%Z)).
+
+  Definition asn_ipe_entry_point {Σ}
+      (segb1 addr : Term Σ ty.wordBits)
+      : Assertion Σ
+    :=
+      asn.formula
+        (formula_relop bop.eq
+           (term_plus 8 (word_times_16 segb1))
+           (term_unsigned addr)).
+
+  Definition asn_unprotected {Σ}
+      (segb1 segb2 : Term Σ ty.wordBits)
+      (am : Term Σ (ty.enum Eaccess_mode))
+      (addr : Term Σ ty.Address)
+      : Assertion Σ
+    :=
+        asn.formula (formula_relop bop.lt
+                       (term_unsigned addr)
+                       (word_times_16 segb1))
+      ∨ asn.formula (formula_relop bop.le
+                       (word_times_16 segb2)
+                       (term_unsigned addr))
+
+      ∨ ( am = term_enum Eaccess_mode X
+        ∗ asn_ipe_entry_point segb1 addr).
+
+  Definition asn_mpu_registers {Σ} : Assertion Σ :=
+      ∃ "MPUCTL0_reg"    , MPUCTL0_reg    ↦ term_var "MPUCTL0_reg"
+    ∗ ∃ "MPUCTL1_reg"    , MPUCTL1_reg    ↦ term_var "MPUCTL1_reg"
+    ∗ ∃ "MPUSEGB2_reg"   , MPUSEGB2_reg   ↦ term_var "MPUSEGB2_reg"
+    ∗ ∃ "MPUSEGB1_reg"   , MPUSEGB1_reg   ↦ term_var "MPUSEGB1_reg"
+    ∗ ∃ "MPUSAM_reg"     , MPUSAM_reg     ↦ term_var "MPUSAM_reg".
+
+  Definition SepContractFun {Δ τ} (f : Fun Δ τ) : Type :=
+    SepContract Δ τ.
+
+  Definition SepContractFunX {Δ τ} (f : FunX Δ τ) : Type :=
+    SepContract Δ τ.
+
+  Definition SepLemma {Δ} (f : Lem Δ) : Type :=
+    Lemma Δ.
+
+  (* Lemmas *)
+
+  Definition lemma_extract_accessible_ptsto : SepLemma extract_accessible_ptsto :=
+    {|
+      lemma_logic_variables := ["addr" :: ty.Address; "m" :: ty.enum Eaccess_mode];
+      lemma_patterns := [term_var "addr"; term_var "m"];
+      lemma_precondition := ⊤;
+      lemma_postcondition := ⊤;
+    |}.
+
+  Definition lemma_return_accessible_ptsto : SepLemma return_accessible_ptsto :=
+    {|
+      lemma_logic_variables := ["addr" :: ty.Address];
+      lemma_patterns := [term_var "addr"];
+      lemma_precondition := ⊤;
+      lemma_postcondition := ⊤;
+    |}.
+
+  (* useless for now, should be called in fetch, for verification *)
+  Definition lemma_open_ptsto_instr : SepLemma open_ptsto_instr :=
+    {|
+      lemma_logic_variables := ["addr" :: ty.wordBits; "id" :: ty.union Uinstr_or_data];
+      lemma_patterns        := [term_var "addr"];
+      lemma_precondition    := term_var "addr" i↦ term_var "id";
+      lemma_postcondition   :=
+        ∃ "bl", ∃ "bh",
+
+        ( ∃ "i",
+            (term_var "id" = term_union Uinstr_or_data Ki (term_var "i")
+             ∗ term_var "addr" m↦ term_var "bl"
+             ∗ term_var "addr" m↦ term_var "bh"
+             ∗ term_var "bh" @ term_var "bl" ≡ term_var "i")
+
+        ∨
+
+         ∃ "d",
+           (term_var "id" = term_union Uinstr_or_data Kd (term_var "d")
+            ∗ term_var "addr" m↦ term_var "bl"
+            ∗ term_var "addr" m↦ term_var "bh"
+            ∗ term_var "bh" @ term_var "bl" = term_var "d"))
+    |}.
+
+  Definition lemma_close_ptsto_instr : SepLemma close_ptsto_instr :=
+    {|
+      lemma_logic_variables :=
+        [ "addr" :: ty.wordBits; "i" :: ty.union Uast
+        ; "bl" :: ty.byteBits; "bh" :: ty.byteBits
+        ];
+
+      lemma_patterns := [term_var "addr"(* ; term_var "w" *)];
+
+      lemma_precondition := ⊤;
+        (*   term_var "addr" m↦ term_var "bl" *)
+        (* ∗ term_binop bop.bvadd (term_var "addr") (term_val ty.wordBits [bv 1]) *)
+        (*     m↦ term_var "bh" *)
+        (* ∗ term_binop (@bop.bvapp _ 8 8) (term_var "bh") (term_var "bl") *)
+        (*     ≡ term_var "i"; *)
+
+      lemma_postcondition := (* term_var "addr" i↦ term_var "i" *) ⊤;
+    |}.
+
+  (* Foreign function contracts *)
+
+  Definition sep_contract_undefined_bitvector (n : nat) :
+      SepContractFunX (@undefined_bitvector n) :=
+      {|
+        sep_contract_logic_variables := ["_" :: ty.int];
+        sep_contract_localstore      := [term_var "_"];
+        sep_contract_precondition    := ⊤;
+        sep_contract_result          := "v";
+        sep_contract_postcondition   := ⊤;
+      |}.
+
+  Definition sep_contract_read_ram :
+    SepContractFunX read_ram :=
+    {|
+      sep_contract_logic_variables := ["addr" :: ty.Address; "v" :: ty.byteBits];
+      sep_contract_localstore      := [term_var "addr"];
+      sep_contract_precondition    := term_var "addr" m↦ term_var "v";
+      sep_contract_result          := "w";
+      sep_contract_postcondition   :=
+        term_var "v" = term_var "w" ∗ term_var "addr" m↦ term_var "v";
+    |}.
+
+  Definition sep_contract_write_ram :
+    SepContractFunX write_ram :=
+    {|
+      sep_contract_logic_variables :=
+        ["addr" :: ty.Address; "v" :: ty.byteBits; "w" :: ty.byteBits];
+
+      sep_contract_localstore      := [term_var "addr"; term_var "v"];
+      sep_contract_precondition    := term_var "addr" m↦ term_var "w";
+      sep_contract_result          := "u";
+      sep_contract_postcondition   :=
+        term_var "addr" m↦ term_var "v"
+        ∗ term_var "u" = term_val ty.unit tt;
+    |}.
+
+  (* Sail function contracts *)
+
+  Definition sep_contract_fetch : SepContractFun fetch :=
+    {|
+      sep_contract_logic_variables :=
+        [ "ipectl" :: ty.wordBits; "segb1" :: ty.wordBits; "segb2" :: ty.wordBits
+        ; "pc_old" :: ty.wordBits; "id" :: ty.union Uinstr_or_data
+        ; "u" :: ty.unit ];
+
+      sep_contract_localstore := [ term_var "u" ];
+
+      sep_contract_precondition :=
+          PC_reg         ↦ term_var "pc_old"
+        ∗ MPUIPC0_reg    ↦ term_var "ipectl"
+        ∗ MPUIPSEGB1_reg ↦ term_var "segb1"
+        ∗ MPUIPSEGB2_reg ↦ term_var "segb2"
+        ∗ asn_mpu_registers
+
+        (* ∗ asn_ipe_configured  (term_var "ipectl") *)
+        (* ∗ asn_untrusted *)
+        (*     (term_var "segb1") (term_var "segb2") (term_var "pc_old") *)
+
+        ∗ term_var "pc_old" i↦ term_var "id";
+
+      sep_contract_result          := "v";
+      sep_contract_postcondition   :=
+          MPUIPC0_reg    ↦ term_var "ipectl"
+        ∗ MPUIPSEGB1_reg ↦ term_var "segb1"
+        ∗ MPUIPSEGB2_reg ↦ term_var "segb2"
+        ∗ asn_mpu_registers
+
+        ∗ PC_reg ↦ term_var "pc_old" +' 2
+
+        ∗ term_var "pc_old" i↦ term_var "id"
+        ∗ ∃ "w",
+          ( term_var "v" = term_union Uwordbyte Kword (term_var "w")
+
+          ∗ ( ∃ "i", ( term_var "id" = term_union Uinstr_or_data Ki (term_var "i")
+                     ∗ term_var "w" ≡ term_var "i")
+            ∨ term_var "id" = term_union Uinstr_or_data Kd (term_var "w")));
+
+      (* encodes_instr is duplicable *)
+
+        (* ∗ ∃ "pc_new", *)
+        (*   ( term_var "pc_new" = term_word_plus [bv 2] (term_var "pc_old") *)
+        (*     ∗ PC_reg ↦ term_var "pc_new" *)
+        (*     ∗ asn_untrusted *)
+        (*         (term_var "segb1") (term_var "segb2") (term_var "pc_new")); *)
+    |}.
+
+  Definition sep_contract_decode : SepContractFunX decode :=
+    {|
+      sep_contract_logic_variables :=
+        [ "wb" :: ty.union Uwordbyte; "w" :: ty.wordBits; "i" :: ty.union Uast];
+      sep_contract_localstore := [term_var "wb"];
+
+      sep_contract_precondition    :=
+          term_var "wb" = term_union Uwordbyte Kword (term_var "w")
+        ∗ term_var "w" ≡ term_var "i";
+
+      sep_contract_result          := "r";
+      sep_contract_postcondition   := term_var "r" = term_var "i";
+    |}.
+
+
+  Definition CEnv : SepContractEnv :=
+    fun Δ τ f =>
+      match f with
+      | fetch => Some sep_contract_fetch
+      | _ => None
+      end.
+
+  Definition CEnvEx : SepContractEnvEx :=
+    fun Δ τ f =>
+      match f with
+      | decode => sep_contract_decode
+      | read_ram => sep_contract_read_ram
+      | write_ram => sep_contract_write_ram
+      | @undefined_bitvector n => sep_contract_undefined_bitvector n
+      end.
+
+  Definition LEnv : LemmaEnv :=
+    fun Δ l =>
+      match l with
+      | extract_accessible_ptsto => lemma_extract_accessible_ptsto
+      | return_accessible_ptsto => lemma_return_accessible_ptsto
+      | open_ptsto_instr => lemma_open_ptsto_instr
+      | close_ptsto_instr => lemma_close_ptsto_instr
+      end.
+End MSP430BlockVerifSpec.
+
+Module MSP430BlockVerifShalExecutor :=
+  MakeShallowExecutor MSP430Base MSP430Signature MSP430Program MSP430BlockVerifSpec.
+Module MSP430BlockVerifExecutor :=
+  MakeExecutor MSP430Base MSP430Signature MSP430Program MSP430BlockVerifSpec.
