src/verification/BlockVer/Verifier.v
@@ -1,0 +1,192 @@
+From Coq Require Import
+     Classes.Morphisms_Prop
+     ZArith.ZArith
+     Lists.List
+     micromega.Lia
+     Strings.String.
+From Equations Require Import
+     Equations.
+From Katamaran Require Import
+     Iris.Instance
+     Iris.Base
+     Notations
+     Semantics
+     Bitvector
+     Refinement.Monads
+     Sep.Hoare
+     Specification
+     Symbolic.Propositions
+     Symbolic.Solver
+     Symbolic.Worlds
+     MicroSail.ShallowExecutor
+     MicroSail.ShallowSoundness
+     MicroSail.SymbolicExecutor
+     MicroSail.RefineExecutor
+     MicroSail.Soundness.
+From iris.base_logic Require lib.gen_heap lib.iprop invariants.
+From iris.bi Require interface big_op.
+From iris.algebra Require dfrac.
+From iris.program_logic Require weakestpre adequacy.
+From iris.proofmode Require string_ident tactics.
+From stdpp Require namespaces.
+
+From MSP430 Require Import Machine Sig BlockVer.Spec.
+
+Import MSP430Program.
+Import Assembly.
+
+Set Implicit Arguments.
+Import ctx.resolution.
+Import ctx.notations.
+Import env.notations.
+Import bv.notations.
+Import ListNotations.
+Open Scope string_scope.
+Open Scope ctx_scope.
+Open Scope Z_scope.
+
+Section BlockVerificationDerived.
+
+  Import MSP430BlockVerifExecutor.
+  Import MSP430BlockVerifShalExecutor.
+
+  (*
+  Definition safeE {Σ} : 𝕊 Σ -> Prop :=
+    fun P => VerificationConditionWithErasure (Erasure.erase_symprop P).
+
+  Definition safeE_safe (p : 𝕊 wnil) (ι : Valuation wnil) : safeE p -> SymProp.safe p [].
+  Proof.
+    unfold safeE.
+    destruct 1 as [H].
+    now apply Erasure.erase_safe'.
+  Qed.
+  *)
+
+  Local Notation "r m↦ v" := (asn.chunk (chunk_user ptstomem [r; v])) (at level 70).
+  Local Notation "r i↦ v" := (asn.chunk (chunk_user ptstoinstr [r; v])) (at level 70).
+
+  Local Notation "v +' n" :=  (term_binop bop.bvadd v (term_val ty.wordBits [bv n])) (at level 50).
+
+  Definition instr_size (i : ast) : bv 16  :=
+    let aux : AM -> bv 16 :=
+      fun am =>
+        match am with
+        | REGISTER_MODE
+        | INDIRECT_REGISTER_MODE
+        | INDIRECT_AUTOINCREMENT_MODE => [bv 0]
+        | INDEXED_MODE => [bv 2]
+        end%N
+    in
+    bv.add
+      (match i with
+       | DOUBLEOP _ _ _ am1 _ am2 => bv.add (aux am1) (aux am2)
+       | SINGLEOP _ _ am _ => aux am
+       | JUMP _ _ | DOESNOTUNDERSTAND _ => [bv 0]
+       end) [bv 2].
+
+  Section Symbolic.
+
+    Import ModalNotations.
+    Import SStoreSpec (evalStoreSpec).
+    Import SHeapSpec SHeapSpec.notations.
+    Import asn.notations.
+
+
+    Definition ptstoinstr_with_args {Σ} addr (i : ast_with_args) : Assertion Σ :=
+      addr i↦ term_val (ty.union Uinstr_or_data) (I (instr_without_args i))
+      ∗ match i with
+        | I0 _     => ⊤
+        | I1 _ a   => addr +' 2 i↦ term_val (ty.union Uinstr_or_data) (D a)
+        | I2 _ a b =>
+              addr +' 2 i↦ term_val (ty.union Uinstr_or_data) (D a)
+            ∗ addr +' 4 i↦ term_val (ty.union Uinstr_or_data) (D b)
+        end.
+
+    Definition exec_instruction_prologue (i : ast_with_args) :
+      Assertion ([ctx] ▻ ("a":: ty.Address))
+    :=
+        PC_reg ↦ term_var "a"
+      ∗ ptstoinstr_with_args (term_var "a") i.
+
+    (* ∃ "an", nextpc ↦ term_var "an" *) (* TODO what is nextpc? *)
+
+    Definition exec_instruction_epilogue (i : ast_with_args) :
+      Assertion ([ctx] ▻ ("a":: ty.Address) ▻ ("na":: ty.Address))
+    :=
+        PC_reg ↦ term_var "na"
+      ∗ ptstoinstr_with_args (term_var "a") i.
+  
+      (* ∗ nextpc ↦ term_var "na" *)
+
+  End Symbolic.
+
+  Section Shallow.
+
+    Import CStoreSpec (evalStoreSpec).
+    Import CHeapSpec CHeapSpec.notations.
+
+    Definition cexec_instruction (i : ast_with_args) :
+      Val ty.Address -> CHeapSpec (Val ty.Address) :=
+      let inline_fuel := 10%nat in
+      fun a =>
+        _ <- produce (exec_instruction_prologue i)
+               [env].["a"∷_ ↦ a] ;;
+        w <- evalStoreSpec (cexec inline_fuel (FunDef fetch))
+               [env].["_ж716"∷_ ↦ tt] ;;
+        d <- cexec_call_foreign decode
+               [env].["w"∷_ ↦ w] ;;
+        _ <- evalStoreSpec (cexec inline_fuel (FunDef execute))
+               [env].["merge#var"∷_ ↦ d] ;;
+        na <- angelic _ ;;
+        _ <- consume
+               (exec_instruction_epilogue i)
+               [env].["a"∷ty.Address ↦ a].["na"∷_ ↦ na] ;;
+        pure na.
+
+    Fixpoint cexec_block_addr (b : list ast_with_args) :
+      Val ty.Address -> Val ty.Address -> CHeapSpec (Val ty.Address) :=
+      fun ainstr apc =>
+        match b with
+        | nil       => pure apc
+        | cons i b' =>
+            _ <- assert_formula (ainstr = apc) ;;
+            apc' <- cexec_instruction i apc ;;
+            cexec_block_addr b'
+              (bv.add ainstr (instr_size (instr_without_args i)))
+              apc'
+        end.
+
+    Definition cexec_double_addr {Σ : LCtx}
+      (req : Assertion (Σ ▻ "a"∷ty.Address)) (b : list ast_with_args) :
+      CHeapSpec (Val ty.Address) :=
+      δ <- demonic_ctx Σ ;;
+      an <- demonic _ ;;
+      _ <- produce req δ.["a"∷ty.Address ↦ an] ;;
+      cexec_block_addr b an an.
+
+    Definition cexec_triple_addr {Σ : LCtx}
+      (req : Assertion (Σ ▻ "a"∷ty.Address)) (b : list ast_with_args)
+      (ens : Assertion (Σ ▻ "a"∷ty.Address ▻ "an"∷ty.Address)) :
+      CHeapSpec unit :=
+      lenv <- demonic_ctx Σ ;;
+      a    <- demonic _ ;;
+      _    <- produce req lenv.["a"∷ty.Address ↦ a]  ;;
+      na   <- cexec_block_addr b a a ;;
+      consume ens lenv.["a"∷ty.Address ↦ a].["an"∷ty.Address ↦ na].
+
+    Definition cblock_verification_condition {Σ : LCtx}
+      (req : Assertion (Σ ▻ "a"∷ty.Address)) (b : list ast_with_args)
+      (ens : Assertion (Σ ▻ "a"∷ty.Address ▻ "an"∷ty.Address)) : Prop
+    := CHeapSpec.run (cexec_triple_addr req b ens).
+
+    Import (hints) CStoreSpec.
+
+    #[export] Instance mono_cexec_instruction {i a} :
+      Monotonic (MHeapSpec eq) (cexec_instruction i a).
+    Proof. typeclasses eauto. Qed.
+
+    #[export] Instance mono_cexec_block_addr {instrs ainstr apc} :
+      Monotonic (MHeapSpec eq) (cexec_block_addr instrs ainstr apc).
+    Proof. revert ainstr apc. induction instrs; cbn; typeclasses eauto. Qed.
+  End Shallow.
+End BlockVerificationDerived.
